src/Framework/Simulation/RefinementLift.v
@@ -1,48 +1,78 @@
 Require Import Primitives Layer Simulation.Definitions.
 
 Section RefinementLift.
-  Variable O1 O2: Operation.
-  Variable L1: Language O1.
-  Variable L2: Language O2.
-  Variable OpRefinement : OperationRefinement L1 O2.
+  Variable O_imp O_abs: Operation.
+  Variable L_imp: Language O_imp.
+  Variable L_abs: Language O_abs.
+  Variable OpRefinement : OperationRefinement L_imp O_abs.
 
-  Fixpoint compile T (p2: prog L2 T) : prog L1 T.
+  Fixpoint compile T (p2: prog L_abs T) : prog L_imp T.
     destruct p2.
     exact (OpRefinement.(compile_op) p).
     exact (Ret t).
     exact (Bind (compile T p2) (fun x => compile T' (p x))).
   Defined.
 
-  Fixpoint oracle_refines_to T (d1: state L1) (p: prog L2 T) o1 o2 : Prop :=
+  Fixpoint oracle_refines_to T (d1: state L_imp) (p: prog L_abs T) o1 o2 : Prop :=
     match p with    
     |Op _ op =>
      exists o2',
-     o2 =  [OpOracle O2 o2' ] /\
+     o2 =  [OpOracle O_abs o2' ] /\
      OpRefinement.(oracle_refines_to_op) d1 op o1 o2'
 
     | Ret v =>
       (exists d1',
-         exec L1 o1 d1 (Ret v) (Crashed d1') /\
+         exec L_imp o1 d1 (Ret v) (Crashed d1') /\
          o2 = [Crash _]) \/
       (exists d1' r,
-         exec L1 o1 d1 (Ret v) (Finished d1' r) /\
+         exec L_imp o1 d1 (Ret v) (Finished d1' r) /\
          o2 = [Cont _])
 
     | @Bind _ T1 T2 p1 p2 =>
       exists o1' o1'' o2' o2'',
       o1 = o1'++o1'' /\
       o2 = o2' ++ o2'' /\
-     ((exists d1', exec L1 o1' d1 (compile T1 p1) (Crashed d1') /\
+     ((exists d1', exec L_imp o1' d1 (compile T1 p1) (Crashed d1') /\
          oracle_refines_to T1 d1 p1 o1' o2') \/
       (exists d1' r ret,
-         exec L1 o1' d1 (compile T1 p1) (Finished d1' r) /\
-         exec L1 o1'' d1' (compile T2 (p2 r)) ret /\
+         exec L_imp o1' d1 (compile T1 p1) (Finished d1' r) /\
+         exec L_imp o1'' d1' (compile T2 (p2 r)) ret /\
          oracle_refines_to T1 d1 p1 o1' o2' /\
          oracle_refines_to T2 d1' (p2 r) o1'' o2''
          ))
     end.
+  (*
+  Theorem exec_preserves_refinement:
+    forall T (p: L_abs.(prog) T) o s_abs ret,
+      (exists s_imp, OpRefinement.(refines_to_op) s_imp s_abs) ->
+      L_abs.(exec) o s_abs p ret ->
+      (exists s_imp', OpRefinement.(refines_to_op) s_imp' (extract_state ret)).
+  Proof.
+    induction p; simpl; intros;
+    invert_exec; eauto;
+    try solve [eapply OpRefinement.(exec_preserves_refinement_op); eauto].
+
+    split_ors; cleanup; eauto.
+    edestruct IHp; eauto.
+  Qed.
+   *)
   
-  Definition LiftRefinement : Refinement L1 L2 := Build_Refinement compile OpRefinement.(refines_to_op) oracle_refines_to.
+  Theorem exec_compiled_preserves_refinement:
+    forall T (p: L_abs.(prog) T) o s_imp ret,
+      (exists s_abs, OpRefinement.(refines_to_op) s_imp s_abs) ->
+      L_imp.(exec) o s_imp (compile T p) ret ->
+      (exists s_abs', OpRefinement.(refines_to_op) (extract_state ret) s_abs').
+  Proof.
+    induction p; simpl; intros;
+    try invert_exec; eauto;
+    try solve [eapply OpRefinement.(exec_compiled_preserves_refinement_op); eauto].
+
+    split_ors; cleanup; eauto.
+    edestruct IHp; eauto.
+  Qed.
+  
+  Definition LiftRefinement : Refinement L_imp L_abs := Build_Refinement compile OpRefinement.(refines_to_op) oracle_refines_to (* exec_preserves_refinement *)
+exec_compiled_preserves_refinement.
 
 End RefinementLift.
 
