src/Refinements/LogCacheToLoggedDisk/Definitions.v
@@ -1,4 +1,5 @@
 Require Import Framework CachedDiskLayer LoggedDiskLayer Log LogCache.
+Require Import FSParameters FunctionalExtensionality Lia.
 Close Scope predicate_scope.
 Import ListNotations.
 
@@ -11,6 +12,7 @@ Definition compile T (p2: Operation.prog high_op T) : prog low T.
  destruct p2.
  exact (read a).
  exact (write l l0).
+ exact recover.
 Defined.
 
 Definition oracle_refines_to T (d1: state low) (p: Operation.prog high_op T) o1 o2 : Prop :=
@@ -40,13 +42,718 @@ Definition oracle_refines_to T (d1: state low) (p: Operation.prog high_op T) o1 
         (exec low o1 d1 (write la lv) (Crashed d1') /\
          o2 = [CrashAfter] /\
          d1' <> d1)
-     )  
+     )
+   | Recover =>
+     (exists d1',
+        exec low o1 d1 recover (Finished d1' tt) /\
+        o2 = [Cont] /\
+        d1' = d1) \/
+     (exists d1',
+        exec low o1 d1 recover (Crashed d1') /\
+        o2 = [CrashBefore] /\
+        d1 = d1')
    end.
 
   Definition refines_to (d1: state low) (d2: state high) :=
     exists F d2' log_state,
       cached_log_rep F d2' d1 log_state /\
       d2 = mem_map fst d2'.
+
+
+  (** refinement preservation **)
+    Lemma nil_or_app:
+    forall T (l: list T),
+      l = [] \/ exists t l', l = l'++[t].
+    intros.
+    eapply rev_ind with (P:= fun l => l = [] \/ (exists (t : T) (l' : list T), l = l' ++ [t])); simpl; eauto.
+  Qed.
+
+  Lemma upd_batch_app:
+    forall A AEQ V l1 l2 l3 l4 (m: @mem A AEQ V),
+      length l1 = length l3 ->
+      upd_batch m (l1++l2) (l3++l4) = upd_batch (upd_batch m l1 l3) l2 l4.
+  Proof.
+    induction l1; simpl; intros; eauto;
+    destruct l3; simpl in *; try lia; eauto.
+  Qed.
+
+  Lemma mem_map_upd_comm:
+    forall A AEQ V1 V2 (m: @mem A AEQ V1) a v (f: V1 -> V2),
+      mem_map f (upd m a v) = upd (mem_map f m) a (f v).
+  Proof.
+    intros. unfold mem_map.
+    extensionality x.
+    destruct (AEQ a x); subst;
+    [ repeat rewrite upd_eq; eauto
+    | repeat rewrite upd_ne; eauto].
+  Qed.
+
+  Definition sumbool_agree {A B C D} (eq1: {A}+{B})(eq2: {C}+{D}):=
+    if eq1 then
+      if eq2 then
+        True
+      else
+        False
+    else
+      if eq2 then
+        False
+      else
+        True.
+
+  Lemma upd_shift_comm:
+    forall A AEQ V (m: @mem A AEQ V) (f: A -> A) a v,
+      (forall x y, sumbool_agree (AEQ x y) (AEQ (f x) (f y))) ->
+      upd (shift f m) a v = shift f (upd m (f a) v).
+  Proof.
+    unfold sumbool_agree; intros; simpl.
+    extensionality x; simpl.
+    specialize (H a x).
+    unfold shift.
+    destruct (AEQ a x);
+    destruct (AEQ (f a) (f x)); subst; intuition;
+    [ repeat rewrite upd_eq
+    | repeat rewrite upd_ne]; eauto.
+  Qed.
+
+  Lemma upd_merge_set_cons_comm:
+    forall A AEQ V (m1: @mem A AEQ V) m2 a v0 v1 vl,
+      upd (merge_set m1 m2) a (v0, v1::vl) = merge_set (upd m1 a v0) (upd m2 a (v1, vl)).
+  Proof.
+    unfold merge_set; intros.
+    extensionality x; simpl.
+    destruct (AEQ a x); subst; intuition;
+    [ repeat rewrite upd_eq
+    | repeat rewrite upd_ne]; eauto.
+  Qed.
+
+  Lemma upd_batch_write_all_mem_map:
+    forall V l l0 (m: @mem addr addr_dec (V * list V)),
+      (forall a, In a l -> m a <> None) ->
+      upd_batch (mem_map fst m) l l0 = mem_map fst (write_all m l l0).
+  Proof.
+    induction l; simpl; intros; eauto.
+    destruct l0; simpl; eauto.
+    specialize (H a) as Hx.
+    destruct (m a); simpl in *; eauto.
+    erewrite <- IHl.
+    rewrite mem_map_upd_comm; simpl; eauto.
+    intros.
+    destruct (addr_dec a a0);
+    [ rewrite upd_eq
+    | rewrite upd_ne ]; eauto; congruence.
+
+    exfalso; apply Hx; eauto.
+  Qed.    
+
+  Lemma write_all_shift_comm:
+    forall V l l0 (m: @mem _ _ (V * list V)) f,
+      (forall x y, sumbool_agree (addr_dec x y) (addr_dec (f x) (f y))) ->
+      write_all (shift f m) l l0 =
+      shift f (write_all m (map f l) l0).
+  Proof.
+    induction l; simpl; intros; eauto.
+    destruct l0; eauto.
+    unfold shift at 1.
+    destruct (m (f a)); eauto.
+    rewrite <- IHl; eauto.
+    rewrite upd_shift_comm; eauto.
+  Qed.
+
+  Lemma write_all_app:
+    forall V l1 l2 l3 l4 (m: @mem _ _ (set V)),
+      length l1 = length l3 ->
+      (forall a, In a l1 -> m a <> None) ->
+      write_all m (l1++l2) (l3++l4) = write_all (write_all m l1 l3) l2 l4.
+  Proof.
+    induction l1; simpl; intros; cleanup; eauto.
+    destruct l3; simpl in *; try lia. 
+    destruct_fresh (m a); simpl; eauto.
+    rewrite IHl1; eauto.
+    intros.
+    destruct (addr_dec a a0);
+    [ repeat rewrite upd_eq in *
+    | repeat rewrite upd_ne in *]; eauto; congruence.
+    exfalso; eapply H0; intuition cleanup.
+  Qed.
+
+  
+  Lemma merge_set_some_l:
+    forall AT AEQ V (m1: @mem AT AEQ V) m2 a v,
+      m1 a = Some v ->
+      m2 a <> None ->
+      exists vs, merge_set m1 m2 a = Some vs /\
+            fst vs = v.
+  Proof.
+    unfold merge_set; simpl; intros.
+    cleanup.
+    destruct (m2 a); try congruence; eauto.    
+  Qed.
+  
+  Lemma merge_set_some_r:
+    forall AT AEQ V (m1: @mem AT AEQ V) m2 a,
+      m1 a = None ->
+      merge_set m1 m2 a = m2 a.
+  Proof.
+    unfold merge_set; simpl; intros.
+    cleanup; eauto.
+  Qed.
+
+  
+  Lemma cached_log_rep_cache_read :
+    forall F s2 s1 a v log_state,
+      cached_log_rep F s2 s1 log_state ->
+      fst s1 (data_start + a) = Some v ->
+      Disk.read s2 a = Some v.
+  Proof.
+    unfold cached_log_rep, Disk.read; intros.
+    cleanup; unfold shift; simpl in *.
+    eapply merge_set_some_l in H0; eauto; cleanup.
+    rewrite H0; eauto.
+    eapply H1.
+    congruence.
+  Qed.
+  
+  Lemma cached_log_rep_disk_read :
+    forall F s2 s1 a log_state,
+      cached_log_rep F s2 s1 log_state ->
+      fst s1 (data_start + a) = None ->
+      Disk.read s2 a = Disk.read (snd (snd s1)) (data_start + a).
+  Proof.
+    unfold cached_log_rep, Disk.read; intros.
+    unfold shift in *; simpl; cleanup.
+    erewrite merge_set_some_r; eauto.
+  Qed.
+
+  Lemma mem_map_fst_some_elim:
+      forall A AEQ V1 V2 (m: @mem A AEQ (V1 * V2)) a v vs,
+        m a = Some (v, vs) ->
+        mem_map fst m a = Some v.
+  Proof.
+    intros.
+    unfold mem_map; simpl; cleanup; eauto.
+  Qed.
+
+  Lemma mem_map_fst_some_exists:
+      forall A AEQ V1 V2 (m: @mem A AEQ (V1 * V2)) a v,
+        mem_map fst m a = Some v ->
+        exists vs, m a = Some (v, vs).
+  Proof.
+    intros.
+    unfold mem_map in *; simpl; cleanup; eauto.
+    destruct p; simpl in *; eauto.
+  Qed.
+
+
+  Lemma upd_batch_not_in_none:
+    forall A AEQ V l l' (m: @mem A AEQ V) a,
+      m a = None ->
+      ~ In a l ->
+      length l = length l' ->
+      upd_batch m l l' a = None.
+  Proof.
+    induction l; simpl; intros; eauto.
+    destruct l'; simpl in *; cleanup; try lia.
+    destruct (AEQ a a0); subst.
+    exfalso; apply H0; intuition.
+    apply IHl.
+    rewrite upd_ne; eauto.
+    intros Hx; apply H0; eauto.
+    lia.
+  Qed.
+  
+  Lemma write_all_merge_set:
+    forall V l l0 (m: @mem _ _ (set V)),
+      NoDup l ->
+      length l = length l0 ->
+      (forall a : addr, In a l -> m a <> None) ->
+      write_all m l l0 =
+      merge_set (upd_batch empty_mem l l0) m.
+  Proof.
+    intros V l.
+    apply rev_ind with
+        (P:= fun l => forall (l0 : list V) (m : mem),
+                     NoDup l ->
+                     length l = length l0 ->
+                     (forall a : addr, In a l -> m a <> None) ->
+                     write_all m l l0 = merge_set (upd_batch empty_mem l l0) m).
+    - simpl; intros; eauto.
+
+    - simpl; intros.
+      destruct (nil_or_app _ l1); subst; simpl.
+      destruct (l0 ++ [x]); simpl; eauto.
+      cleanup; subst.
+      repeat rewrite app_length in H1; simpl in *.
+      apply NoDup_app_l in H0 as Hx.
+      rewrite upd_batch_app; simpl; try lia.
+      rewrite write_all_app; try lia.
+      rewrite H; eauto; try lia.
+      simpl.
+      destruct_fresh (merge_set (upd_batch empty_mem l0 x1) m x).
+      setoid_rewrite upd_merge_set_cons_comm.
+      setoid_rewrite upd_nop at 2; eauto.
+      destruct p; simpl.
+      rewrite merge_set_some_r in D; eauto.      
+      eapply upd_batch_not_in_none; eauto.
+      apply NoDup_app_comm in H0; simpl in *.
+      inversion H0; eauto.
+      lia.
+      rewrite merge_set_some_r in D; eauto.
+      exfalso; eapply H2; eauto.
+      apply in_app_iff; simpl; eauto.
+
+      eapply upd_batch_not_in_none; eauto.
+      apply NoDup_app_comm in H0; simpl in *.
+      inversion H0; eauto.
+      lia.
+      intros; eapply H2; eauto.
+  Qed.
+
+  Lemma refines_to_upd_batch:
+    forall l l0 s1 s2,
+      NoDup l ->
+      length l = length l0 ->
+      refines_to s1 s2 ->
+      exists s1', refines_to s1' (upd_batch s2 l l0).
+  Proof.
+    intros.
+    unfold refines_to in *; cleanup.
+    eexists; exists x, (write_all x0 l l0).
+    exists x1.
+    rewrite upd_batch_write_all_mem_map.
+    split; eauto.
+  Abort.
+
+  (*
+    Lemma cached_log_rep_upd_cons:
+      forall l l0 F d s log_state,
+        cached_log_rep F d s log_state ->
+        NoDup l ->
+        length l = length l0 ->
+        exists s', cached_log_rep F (write_all d l l0) s' log_state.
+    Proof.
+      intros. 
+      unfold cached_log_rep in H; cleanup.
+      rewrite <- H in *.
+      unfold cached_log_rep; simpl.
+      destruct s, s0; simpl in *.
+      do 3 eexists.
+      repeat split.
+      
+      5: rewrite write_all_shift_comm, write_all_merge_set.
+      instantiate (2:= (upd_batch s (map (Init.Nat.add data_start) l) l0, (s0, s1))).
+      all: simpl; eauto.
+      
+      
+      eauto.
+      
+      cleanup; eauto.
+      
+      unfold merge_set at 1.
+      destruct_fresh (m1 a).
+      destruct_fresh (m2 a); simpl.
+      unfold upd_disk.
+      setoid_rewrite upd_merge_set_cons_comm.
+      rewrite IHl.
+      Search merge_set.
+      destruct (m (f a)); eauto.
+      rewrite <- IHl; eauto.
+      unfold upd_disk;
+      rewrite upd_shift_comm; eauto.
+    Qed.
+    
+    rewrite write_all_merge_set.
+    
+    intros.
+    unfold sumbool_agree.
+    Print Log.txn.
+    exists ({ record : Log.txn_record;  addr_blocks : list value;  data_blocks : list value }++x0).
+    unfold 
+      do 4 eexists.        
+    repeat split.
+    4: eauto.
+
+    
+    eauto.
+
+  Abort.
+
+
+  
+  eapply rev_ind with (P:= fun l =>
+                             forall (l0 : list value) (s1 : state Definitions.low) (s2 : state Definitions.high),
+                               length l = length l0 ->
+                               refines_to s1 s2 -> exists s1' : state Definitions.low, refines_to s1' (upd_batch s2 l l0)); simpl;
+  unfold refines_to; intros; eauto.
+  destruct (nil_or_app _ l1); subst;
+  simpl in *; eauto; cleanup.
+  do 4 eexists; intuition eauto.
+  repeat rewrite app_length in *; simpl in *.
+  
+  rewrite upd_batch_app by lia.
+  edestruct H; eauto; cleanup.
+  instantiate (1:=x1); lia.
+  rewrite H3 in *; clear H3.
+  simpl.
+  destruct_fresh (x7 x).
+  {
+    eexists.
+    exists x6, (upd x7 x (x0, fst p::snd p)).
+    eexists.
+    setoid_rewrite mem_map_upd_comm; split; eauto.
+  Abort.
+  
+
+  Lemma sp_write_batch_to_cache_ok:
+    forall l l0 t s' F log_state hdr txns m,
+      NoDup l ->
+      length l = length l0 ->
+      
+      strongest_postcondition CachedDiskLang (LogCache.write_batch_to_cache l l0)
+        (fun o s =>
+           m = fst s /\
+           (forall a, In a l -> snd (snd s) a <> None ) /\
+           addrs_match (fst s) (snd (snd s)) /\
+           (Log.log_rep log_state hdr txns (fst (snd s)) * F)%predicate (snd (snd s))) t s' ->
+      
+      fst s' = upd_batch m l l0 /\
+      addrs_match (fst s') (snd (snd s')) /\
+      (Log.log_rep log_state hdr txns (fst (snd s')) * F)%predicate (snd (snd s')).
+  Proof.
+    induction l; simpl; intros;
+    cleanup; simpl in *; eauto; try lia.
+
+    cleanup.
+    inversion H; cleanup.
+    apply sp_exists_extract in H1; cleanup.
+    edestruct IHl; eauto; try lia.
+    
+    eapply sp_impl; eauto.
+    simpl; intros; cleanup; intuition eauto.
+    destruct s; simpl in *; cleanup.
+    unfold addrs_match; intros.
+    destruct (addr_dec a a0); subst;
+    [ rewrite upd_eq in H2
+    | rewrite upd_ne in H2 ]; eauto.
+  Qed.
+
+  Lemma and_exists:
+    forall T (P: T -> Prop) (Q: Prop),
+      (exists t, P t) /\ Q -> (exists t, P t /\ Q).
+  Proof.
+    firstorder.
+  Qed.
+  *)
+
+  Set Nested Proofs Allowed.
+   
+  
+  
+  Lemma exec_compiled_preserves_refinement:
+    forall T (p2: high_op.(Operation.prog) T) o1 s1 ret,
+        (exists s2, refines_to s1 s2) ->
+        low.(exec) o1 s1 (compile T p2) ret ->
+        (exists s2', refines_to (extract_state ret) s2').
+  Proof.
+    intros; destruct p2; simpl in *; cleanup.
+    {
+      destruct ret.
+      {
+        unfold read in *; repeat (invert_exec; simpl in *; cleanup);
+        try solve [inversion H5; cleanup;
+                   try inversion H7; cleanup;
+                   eexists; intuition eauto ].
+      }
+      {
+        unfold read in *;
+        repeat (try split_ors; cleanup;
+                invert_exec;
+                simpl in *; cleanup);
+        try solve [
+              inversion H5; cleanup;
+              try inversion H6; cleanup;
+              eexists; intuition eauto].
+      }
+    }
+    {
+      destruct ret.
+      {
+        {
+          unfold write in *; simpl in *.
+          (** TODO: Speed this up **)
+          repeat (cleanup; invert_exec;
+                  simpl in *; cleanup; intuition).
+          repeat
+            match goal with
+            |[H: DiskLayer.exec' _ _ _ _ |- _ ] =>
+             inversion H; clear H; cleanup
+            end.
+
+          repeat
+            match goal with
+            | [H: exec _ _ _ (BatchOperations.hash_all _ _) _ |- _ ] =>
+              eapply BatchOperations.hash_all_finished in H
+            | [H: exec _ _ _ (BatchOperations.read_consecutive _ _) _ |- _ ] =>
+              eapply BatchOperations.read_consecutive_finished in H
+            | [H: exec _ _ _ (BatchOperations.write_consecutive _ _) _ |- _ ] =>
+              unfold BatchOperations.write_consecutive in H;
+              eapply BatchOperations.write_batch_finished in H
+            | [H: exec _ _ _ (BatchOperations.encrypt_all _ _) _ |- _ ] =>
+              eapply BatchOperations.encrypt_all_finished in H
+            end.
+          
+          match goal with
+          | [H: exec _ _ _ (LogCache.write_batch_to_cache _ _) _ |- _ ] =>
+            eapply LogCache.write_batch_to_cache_finished in H
+          end; try logic_clean.
+
+          match goal with
+          | [H: exec _ _ _ (Log.apply_txns _ _) _ |- _ ] =>
+            eapply Log.sp_apply_txns in H
+          end; try logic_clean.
+
+          inversion H19; clear H19; subst; sigT_eq.
+
+          repeat
+            match goal with
+            | [H: context [ fst ?x ] |- _ ] =>
+              destruct x; simpl in *
+            | [H: context [ snd ?x ] |- _ ] =>
+              destruct x; simpl in *
+            end; cleanup_no_match.
+          
+          all: admit.
+        }
+      }
+      { admit. }
+    }
+    {
+      destruct ret.
+      {
+        unfold recover in *; repeat (invert_exec; simpl in *; cleanup).
+
+           repeat
+            match goal with
+            |[H: DiskLayer.exec' _ _ _ _ |- _ ] =>
+             inversion H; clear H; cleanup
+            end.
+
+           repeat
+            match goal with
+            | [H: exec _ _ _ (BatchOperations.hash_all _ _) _ |- _ ] =>
+              eapply BatchOperations.hash_all_finished in H
+            | [H: exec _ _ _ (BatchOperations.read_consecutive _ _) _ |- _ ] =>
+              eapply BatchOperations.read_consecutive_finished in H
+            | [H: exec _ _ _ (BatchOperations.write_consecutive _ _) _ |- _ ] =>
+              unfold BatchOperations.write_consecutive in H;
+              eapply BatchOperations.write_batch_finished in H
+            | [H: exec _ _ _ (BatchOperations.encrypt_all _ _) _ |- _ ] =>
+              eapply BatchOperations.encrypt_all_finished in H
+            end.
+
+        repeat
+          match goal with
+          | [H: context [ fst ?x ] |- _ ] =>
+            destruct x; simpl in *
+          | [H: context [ snd ?x ] |- _ ] =>
+            destruct x; simpl in *
+          end; cleanup_no_match.
+
+        XXX
+
+        subst.
+        intuition subst.
+
+        repeat
+          match goal with
+          |[H: DiskLayer.exec' _ _ _ _ |- _ ] =>
+           inversion H; clear H; cleanup
+          end.
+          
+        try solve [inversion H5; cleanup;
+                   try inversion H7; cleanup;
+                   eexists; intuition eauto ].
+      }
+      {
+        unfold read in *;
+        repeat (try split_ors; cleanup;
+                invert_exec;
+                simpl in *; cleanup);
+        try solve [
+              inversion H5; cleanup;
+              try inversion H6; cleanup;
+              eexists; intuition eauto].
+      }
+    }
+    
+          
+          Search exec.
+          
+          XXX HERE XXX
+          try solve [inversion H5; cleanup;
+                   try inversion H7; cleanup;
+                   eexists; intuition eauto ].
+      }
+      {
+        unfold read in *;
+        repeat (try split_ors; cleanup;
+                invert_exec;
+                simpl in *; cleanup);
+        try solve [
+              inversion H5; cleanup;
+              try inversion H6; cleanup;
+              eexists; intuition eauto].
+      }
+        eapply exec_to_sp with (P := fun o s => refines_to s x /\ s = s1 /\ o = o1) in H0; eauto.
+        unfold write in *; simpl in *;
+        repeat (cleanup; simpl in *).
+
+                
+                
+                 repeat (match goal with
+                        | [H: strongest_postcondition _ _ _ _ _ |- _ ] =>
+                          eapply sp_to_exec in H; cleanup
+                        end).
+                 simpl in *.
+
+                 repeat invert_exec.
+                 Search exec.
+                 
+                2: {
+                  intuition eauto.
+                  apply H1.
+
+   Set Nested Proofs Allowed. 
+   eapply sp_bind in H0.
+                
+                eauto;
+                do 4 eexists; intuition eauto.
+                
+      eapply exec_to_scp with (P := fun o s' => refines_to s' x /\ s' = s1 /\ o = o1) in H0; eauto.
+      simpl in *; repeat (try split_ors; cleanup; simpl in *); eauto;
+      inversion H0; cleanup; eauto;
+      do 4 eexists; intuition eauto.
+    
+                         {
+
+        Lemma sp_write_ok:
+          forall l l0 t s',
+            strongest_postcondition CachedDiskLang (write l l0) (fun o s => exists s2, refines_to s s2) t s' ->
+            exists s2' : state', refines_to s' s2'.
+        Proof.
+          unfold write; intros.
+          repeat cleanup;
+          try solve [ simpl in *; cleanup; eauto].
+          unfold refines_to, cached_log_rep in *.
+          repeat (apply sp_exists_extract in H; cleanup).
+          eapply sp_impl in H; [|simpl; intros o s Hx; eapply and_exists in Hx; apply Hx].
+          repeat (apply sp_exists_extract in H; cleanup).
+          eapply sp_impl in H; [|simpl; intros o s Hx; eapply and_exists in Hx; apply Hx].
+          repeat (apply sp_exists_extract in H; cleanup).
+          
+          Opaque Log.commit.
+          simpl in *;
+          cleanup; simpl in *.
+          apply sp_lift2 in H.
+          simpl in H.
+          
+          eapply sp_impl in H.
+          eapply sp_write_batch_to_cache_ok in H; eauto.
+          cleanup.
+
+          
+          
+             
+            rewrite upd_batch_upd_comm.
+            eapply IHl; eauto; try lia.
+            eapply sp_impl; eauto.
+            simpl; intros; cleanup; eauto.
+            destruct s; simpl in *; cleanup.
+
+              Lemma cached_log_rep_cache_upd:
+                forall d a v p x1 s0 F log_state,
+                d a = Some p ->
+                cached_log_rep F d (x1, s0) log_state -> 
+                cached_log_rep F (upd d a (v, fst p :: snd p)) (upd x1 a v, s0) log_state.
+              Proof.
+                unfold cached_log_rep; simpl; intros; cleanup.
+                repeat split; eauto.
+
+            Lemma refines_to_upd:
+              forall s s0 s2 a v,
+              refines_to (s, s0) s2 ->
+              exists s2', refines_to (upd s a v, s0) s2'.
+            Proof.
+              unfold refines_to in *; simpl; intros; cleanup.
+              unfold cached_log_rep in *; simpl in *; cleanup.
+              do 4 eexists; repeat split.
+              do 2 eexists; repeat split.
+              instantiate {1:= }
+            simpl in *; cleanup; try lia.
+            
+          Search LogCache.write_batch_to_cache.
+          2: {
+            
+        
+        eapply A.
+        eapply exec_to_sp; eauto.
+        
+        assume (A:(forall s',
+                     strongest_crash_postcondition CachedDiskLang (write l l0) (fun o s => exists s2, refines_to s s2) s' ->
+                     exists s2' : state', refines_to s' s2')).
+        eapply A.
+        eapply exec_to_scp; eauto.
+      }
+    }
+
+    {
+      destruct ret.
+      eapply exec_to_sp with (P := fun o s => refines_to s x /\ s = s1) in H0; unfold refines_to in *; eauto.
+      simpl in *; cleanup; simpl; eauto; do 4 eexists; intuition eauto.
+      eapply exec_to_scp with (P := fun o s => refines_to s x /\ s = s1) in H0; unfold refines_to in *; eauto.
+      simpl in *; cleanup; simpl; eauto; do 4 eexists; intuition eauto.
+    }
+    
+    {
+      invert_exec; eauto.
+      split_ors; cleanup; eauto.
+      eapply IHp2 in H1; eauto.
+    }
+Admitted.
+
+(*                          
+Lemma exec_preserves_refinement:
+  exec_preserves_refinement refinement.
+Proof.
+  unfold exec_preserves_refinement; induction p; simpl; intros.
+  destruct ret.
+  {
+    eapply exec_to_sp with (P := fun o s => exists x, refines_to x s) in H0; eauto.
+    destruct p; simpl in *; cleanup; eauto.
+    split_ors; cleanup; eauto.
+    admit. (* Doable *)
+  }
+  {
+    eapply exec_to_scp with (P := fun o s => exists x, refines_to x s) in H0; eauto.
+    destruct p; simpl in *; cleanup; eauto.
+    split_ors; cleanup; eauto.
+    admit. (* Doable *)
+  }
+  
+  destruct ret.
+  {
+    eapply exec_to_sp with (P := fun o s => exists x, refines_to x s) in H0; eauto.
+    simpl in *; cleanup; eauto.
+  }
+  {
+    eapply exec_to_scp with (P := fun o s => exists x, refines_to x s) in H0; eauto.
+  }
+  
+  invert_exec.
+  eapply IHp in H1; eauto; simpl in *.
+  split_ors; cleanup; eauto.
+  eapply IHp in H1; eauto; simpl in *.
+Admitted.
+*)
 
   Definition LoggedDiskOperationRefinement := Build_OperationRefinement compile refines_to oracle_refines_to.
   Definition LoggedDiskRefinement := LiftRefinement LoggedDiskLang LoggedDiskOperationRefinement.
