src/Framework/Layer/Automation.v
@@ -1,0 +1,152 @@
+Require Import Primitives Layer.Operation
+        Layer.Language Layer.HorizontalComposition.
+
+Local Ltac invert_exec'' H :=
+  inversion H; subst; clear H; repeat sigT_eq.
+
+  
+Lemma bind_sep:
+  forall O (L: Language O) T T' o d (p1: prog L T) (p2: T -> prog L T') ret,
+    exec L o d (Bind p1 p2) ret ->
+    match ret with
+    | Finished d' r =>
+    (exists o1 o2 d1 r1,
+       exec L o1 d p1 (Finished d1 r1) /\
+       exec L o2 d1 (p2 r1) ret /\
+       o = o1++o2)
+  | Crashed d' =>
+    (exists o1 o2,
+    o = o1++o2 /\    
+    (exec L o1 d p1 (Crashed d') \/
+     (exists d1 r1,
+        exec L o1 d p1 (Finished d1 r1) /\
+        exec L o2 d1 (p2 r1) ret)))
+    end.
+Proof.
+  intros.
+  invert_exec'' H; eauto.
+  destruct ret.
+  do 2 eexists; eauto.
+  do 2 eexists; split; eauto.
+ Qed.
+
+ Local Lemma lift1_invert_exec :
+    forall O1 O2 (L1: Language O1) (Lc: Language (HorizontalComposition O1 O2))
+      T (p1: L1.(prog) T) (o: Lc.(oracle)) s s' t,
+      exec Lc o s (lift_L1 O2 p1) (Finished s' t) ->
+      exists o1,
+        o = map (fun o =>
+                   match o with
+                   |OpOracle _ o1 =>
+                    OpOracle (HorizontalComposition O1 O2)
+                             [Oracle1 O1 O2 o1]%list
+                   |Language.Cont _ =>
+                    Language.Cont _
+                   |Language.Crash _ =>
+                    Language.Crash _
+                   end) o1 /\
+        snd s = snd s' /\
+        exec L1 o1 (fst s) p1 (Finished (fst s') t).
+  Proof.
+    induction p1; simpl; intros.
+    {      
+      invert_exec'' H.
+      invert_exec'' H5.      
+      eexists; intuition eauto.
+      simpl; eauto.
+    }
+    {
+      invert_exec'' H.
+      eexists; intuition eauto.
+      2: econstructor.
+      simpl; eauto.
+    }
+    {
+      invert_exec'' H0.
+      edestruct IHp1; eauto; cleanup.
+      edestruct H; eauto; cleanup.
+      
+      eexists; intuition eauto.
+      2: econstructor; eauto.
+      rewrite map_app; eauto.
+    }
+  Qed.
+
+    
+Local Lemma lift2_invert_exec :
+    forall O1 O2 (L2: Language O2) (Lc: Language (HorizontalComposition O1 O2))
+      T (p2: L2.(prog) T) (o: Lc.(oracle)) s s' t,
+      exec Lc o s (lift_L2 O1 p2) (Finished s' t) ->
+      exists o2,
+        o = map (fun o =>
+                   match o with
+                   |OpOracle _ o1 =>
+                    OpOracle (HorizontalComposition O1 O2)
+                             [Oracle2 O1 O2 o1]%list
+                   |Language.Cont _ =>
+                    Language.Cont _
+                   |Language.Crash _ =>
+                    Language.Crash _
+                   end) o2 /\
+        fst s = fst s' /\
+        exec L2 o2 (snd s) p2 (Finished (snd s') t).
+  Proof.
+    induction p2; simpl; intros.
+    {
+      invert_exec'' H.
+      invert_exec'' H5.
+      eexists; intuition eauto.
+      simpl; eauto.
+    }
+    {
+      invert_exec'' H.
+      eexists; intuition eauto.
+      2: econstructor.
+      simpl; eauto.
+    }
+    {
+      invert_exec'' H0.
+      edestruct IHp2; eauto; cleanup.
+      edestruct H; eauto; cleanup.
+      
+      eexists; intuition eauto.
+      2: econstructor; eauto.
+      rewrite map_app; eauto.
+    }
+  Qed.
+
+
+  Local Ltac invert_exec' :=
+    match goal with
+    |[H : recovery_exec _ _ _ _ _ _ _ |- _ ] =>
+     invert_exec'' H
+    | [ H: exec _ _ _ ?p _ |- _ ] =>
+      match p with
+      | Bind _ _ => idtac
+      | Op _ _ => invert_exec'' H
+      | Ret _ => invert_exec'' H
+      end
+    | [ H: exec' _ _ ?p _ |- _ ] =>
+      match p with
+      | Bind _ _ => idtac
+      | Op _ _ => invert_exec'' H
+      | Ret _ => invert_exec'' H
+      end
+    | [ H: exec _ _ _ (lift_L1 _ _) (Finished _ _) |- _ ] =>
+      eapply lift1_invert_exec in H; logic_clean
+    | [ H: exec _ _ _ (lift_L2 _ _) (Finished _ _) |- _ ] =>
+      eapply lift2_invert_exec in H; logic_clean
+    | [ H: HorizontalComposition.exec' _ _ _ _ |- _ ] =>
+      invert_exec'' H
+    | [ H: Operation.exec _ _ _ _ _ |- _ ] =>
+      invert_exec'' H
+    end.
+
+  Ltac invert_exec :=
+  invert_exec' ||
+  match goal with
+  |[H : exec _ _ _ (Bind _ _) _ |- _ ] =>
+   apply bind_sep in H; repeat cleanup
+  |[H : exec' _ _ (Bind _ _) _ |- _ ] =>
+   apply bind_sep in H; repeat cleanup
+  end.
