src/Framework/Simulation/Simulation.v
@@ -1,1 +1,1 @@
-Require Export Simulation.Definitions Simulation.WeakestPreconditions Simulation.Metatheory  Simulation.RefinementLift.
+Require Export Simulation.Definitions Simulation.RefinementLift.
