src/Layers/BasicLayers/Disk/DiskLayer.v
@@ -175,7 +175,7 @@ Section DiskLayer.
   Definition DiskOperation :=
     Build_Operation
       (list_eq_dec token_dec')
-      after_crash'
+      (* after_crash' *)
       disk_prog
       exec'
       weakest_precondition'
